src/Soundness.v
@@ -1,5 +1,6 @@
-From TLC Require Import LibString LibLN.
+From TLC Require Import LibString LibList LibLN.
 From MCore Require Import Syntax Typing SmallStep Tactics.
+Import LibListNotation.
 
 Module Soundness (P : PAT).
   Module S := SmallStep P.
@@ -31,8 +32,7 @@ Module Soundness (P : PAT).
           rewrite* Topen_t_open_comm. apply_empty ok_term_comm...
         + rewrite~ open_notin_T. }
       { Case "TmTyLam". rewrite notin_Topen_k in *...
-        assert (ok_kind Gamma k)
-          by (apply_empty~ (ok_kind_tname_strengthening T) ; apply* ok_env_push).
+        assert (ok_kind Gamma k) by apply_empty~ (ok_kind_tname_strengthening T).
         apply_fresh* TTyLam as X.
         forwards~ Htype': H4 X. apply_fresh TType as T'...
         rewrite~ (Tsubst_t_intro T (FTName T')).
@@ -56,11 +56,84 @@ Module Soundness (P : PAT).
     Qed.
 
     Lemma ok_term_Kopen_push :
-      forall Gamma K d ty' T t t' ty,
-        Gamma & K ~ BindCon d ty' T |= Kopen_t 0 (FCon K) t ~: ty ->
+      forall L Gamma d ty' T t t' ty,
+        (forall K, K \notin L ->
+              Gamma & K ~ BindCon d ty' T |= Kopen_t 0 (FCon K) t ~: ty) ->
         push_value (TmConDef d ty' T) t t' ->
         Gamma |= t' ~: ty.
-    Admitted.
+    Proof with eauto with mcore.
+      introv Htype Hpush. gen L ty.
+      remember (TmConDef d ty' T) as f eqn:Hf.
+      induction Hpush ; introv Htype ; substs ;
+        pick_fresh K' ; forwards~ Htype0: Htype K' ;
+        forwards Henv : ok_term_ok_env Htype0 ;
+        forwards (L0 & T' & Heq & Hd & Htk & HT): ok_env_con_inv Henv ;
+        inverts Htype0 ; substs ; simpls.
+      { Case "TmLam". assert (Heq: Kopen_ty 0 (FCon K') ty = ty) by apply~ notin_Kopen_ty.
+        rewrite Heq in *.
+        assert (Gamma |= ty ~:: KiType)
+          by (apply_empty~ (ok_type_con_strengthening K') ; eauto ; apply* ok_env_push).
+        assert (Hty' : forall x X,
+                   X \notin L0 \u dom Gamma \u \{x} ->
+                   x # Gamma ->
+                   Gamma & x ~ BindVar ty & X ~ BindTVar (KiData d) |= {0 ~> TyFVar X} ty' ~:: KiType).
+        { introv Hnin Hfr. forwards~ Htk' : Htk X. apply~ ok_type_weakening.
+          constructor*. constructor~. apply_empty~ ok_data_weakening. constructor*. }
+        apply_fresh* TLam as x.
+        forwards~ Htype': H4 x. apply_fresh TConDef as K...
+        - apply_empty ok_data_weakening...
+        - rewrite~ (Ksubst_t_intro K' (FCon K)).
+          + rewrite~ <- (Ksubst_ty_fresh K' (FCon K)). apply_empty ok_term_Ksubst...
+            rewrite* Kopen_t_open_comm. apply_empty~ ok_term_comm.
+            apply_fresh EnvCon as X... apply_empty~ ok_data_weakening. constructor...
+          + rewrite~ open_notin_K. }
+      { Case "TmTyLam". assert (Heq: Kopen_k 0 (FCon K') k = k) by apply~ notin_Kopen_k.
+        rewrite Heq in *.
+        assert (ok_kind Gamma k) by apply_empty* (ok_kind_con_strengthening K').
+        assert (Heq' : forall x, {1 ~> TyFVar x}ty' = ty').
+        { intros. pick_fresh y. apply topen_neq with (J := 0) (V := TyFVar y)...
+          rewrite~ topen_lct. apply* ok_type_lct. }
+        assert (Hty' : forall x X,
+                   X \notin L0 \u dom Gamma \u \{x} ->
+                   x # Gamma ->
+                   Gamma & x ~ BindTVar k & X ~ BindTVar (KiData d) |= {0 ~> TyFVar X} ty' ~:: KiType).
+        { introv Hnin Hfr. forwards~ Htk' : Htk X. apply~ ok_type_weakening.
+          constructor*. constructor~. apply_empty~ ok_data_weakening. constructor*. }
+        apply_fresh* TTyLam as X.
+        forwards~ Htype': H4 X. apply_fresh TConDef as K...
+        - apply_empty ok_data_weakening...
+        - rewrite~ Heq'.
+        - rewrite Heq'. rewrite~ (Ksubst_t_intro K' (FCon K)).
+          + rewrite~ <- (Ksubst_ty_fresh K' (FCon K)).
+            * apply_empty ok_term_Ksubst... rewrite* Kopen_t_topen_comm. apply_empty~ ok_term_comm.
+              apply_fresh EnvCon as X... apply_empty~ ok_data_weakening. constructor...
+            * rewrite~ topen_notin_K. simpls~.
+          + rewrite~ topen_t_notin_K. }
+      { Case "TmCon". assert (Heq: Kopen_ty 0 (FCon K') ty = ty) by apply~ notin_Kopen_ty.
+        rewrite Heq in *.
+        assert (Htk1 : Gamma |= ty ~:: KiData [ (FTName T0, FCon K0 :: []) ]).
+        { apply_empty* (ok_type_con_strengthening K'). }
+        assert (Hin : K0 \in dom Gamma).
+        { forwards~ Hd' : ok_type_ok_data Htk1. inverts Hd'. inverts H11.
+          applys~ get_some_inv H14. }
+        assert (Hnin : K' # Gamma).
+        { inverts~ Henv. }
+        assert (Hneq : K' <> K0).
+        { intro ; substs ; false. }
+        assert (HeqK : K = FCon K0).
+        { destruct K ; solve_var. }
+        rewrite HeqK.
+        constructors~.
+        + binds_cases H2...
+        + apply_empty (ok_type_con_strengthening K') ; eauto ; apply* ok_env_push.
+        + specializes~ IHHpush __. apply_fresh IHHpush as K1.
+          rewrite~ (Ksubst_t_intro K' (FCon K1)). rewrite~ <- (Ksubst_ty_fresh K' (FCon K1)).
+          * apply_empty~ ok_term_Ksubst.
+          * rewrite~ topen_notin_K. binds_cases H2.
+            forwards (L'&?&?&?&Htk'&?): ok_env_binds_con_inv B. apply* ok_env_push.
+            pick_fresh X. forwards~ Hnin': ok_type_notin_K K' (Htk' X).
+            rewrite~ topen_notin_K in Hnin'. simpls~. }
+    Qed.
 
     Theorem preservation :
       forall Gamma t t' ty,
@@ -83,7 +156,7 @@ Module Soundness (P : PAT).
         apply_empty~ ok_term_tsubst. }
       { Case "TmType". applys* ok_term_Topen_push (L \u Tfv_ty ty). }
       { Case "TmTypeCong". apply_fresh TType as T' ; auto. }
-      { Case "TmConDef". pick_fresh K'. applys* ok_term_Kopen_push K'. }
+      { Case "TmConDef". pick_fresh K'. applys* ok_term_Kopen_push (L \u Kfv_ty ty2). }
       { Case "TmConDefCong". apply_fresh TConDef as K'; auto. }
     Qed.
 
